coq/Lambda.v
@@ -1,36 +1,248 @@
 Require Import List.
 Import ListNotations.
 Require Import Omega.
-Require Import Ascii.
-Require Import String.
-Local Open Scope string_scope.
+Require Import Arith.
+Require Import Id.
 
 Inductive term : Type := 
-  Var  : string -> term
-| Free : string -> term
-| Abs  : string -> term -> term 
+  Var  : id -> term
+| Abs  : id -> term -> term 
 | App  : term -> term -> term.
-
-Definition a (x : string) : term := 
-  match x with
-  | EmptyString => Free x
-  | String h t => 
-     if andb (leb (Ascii.nat_of_ascii "A") (Ascii.nat_of_ascii h)) 
-             (leb (Ascii.nat_of_ascii h) (Ascii.nat_of_ascii "Z")) 
-        then Free x 
-        else Var x
-  end.
 
 Notation "\ x , .. , z --> t" := (Abs x .. (Abs z t) .. ) (at level 38, no associativity).
 Notation "m @ n"              := (App m n) (at level 39, left associativity).
 
-Definition id    := \"x" --> a"x".
-Definition apply := \"f", "x" --> (a"f" @ a"x").
-Definition z     := \"f", "x" --> a"x".
-Definition s     := \"n", "f", "x" --> (a"f" @ (a"n" @ a"f" @ a"x")).
-Definition add   := \"n", "m", "f", "x" --> (a"m" @ a"f" @ (a"n" @ a"f" @ a"x")).
-Definition mul   := \"n", "m", "f", "x" --> (a"m" @ (a"n" @ a"f") @ a"x").
+Definition f := Id 0.
+Definition g := Id 1.
+Definition h := Id 2.
 
+Definition x := Id 3.
+Definition y := Id 4.
 
+Definition m := Id 5.
+Definition n := Id 6.
 
+Definition v i := Var i.
+           
+Definition i     := \ x --> v x.
+Definition apply := \ f, x --> (v f @ v x).
+Definition z     := \ f, x --> v x.
+Definition s     := \ n, f, x --> (v f @ (v n @ v f @ v x)).
+Definition add   := \ n, m, f, x --> (v m @ v f @ (v n @ v f @ v x)).
+Definition mul   := \ n, m, f, x --> (v m @ (v n @ v f) @ v x).
 
+Inductive fv : id -> term -> Prop :=
+  fv_Var : forall x,  fv x (v x)
+| fv_Abs : forall x y t,  fv y t -> x <> y -> fv y (\ x --> t)
+| fv_App : forall x a b,  (fv x a) \/ (fv x b) -> fv x (a @ b).
+
+Lemma fv_var: forall x y, fv x (v y) -> x = y.
+Proof. intros x y H. inversion H. auto. Qed.
+(*
+Reserved Notation "m [[ x <~ y ]] n" (at level 40, left associativity).
+
+Inductive cas : term -> id -> id -> term -> Prop :=
+  cas_Var     : forall x y           , (v x) [[x <~ y]] (v y)
+| cas_Var_neq : forall x y z         , x <> z -> (v z) [[x <~ y]] (v z)
+| cas_App     : forall m n m' n' x y , m [[ x <~ y ]] m' -> n [[ x <~ y ]] n' -> (m @ n) [[ x<~ y ]] (m' @ n')
+| cas_Lam     : forall m x y         , (\ x --> m) [[ x <~ y ]] (\x --> m)
+| cas_Lam_neq : forall m m' x y z    , z <> x -> z <> y -> m [[ x<~ y ]] m' -> (\ z --> m) [[ x <~ y ]] (\z --> m')
+| cas_Lam_ren : forall m m' m'' x y z, ~ fv z m -> m [[ y <~ z ]] m' -> m' [[ x <~ y ]] m'' -> (\y --> m) [[ x <~ y ]] (\ z --> m'')
+where "m [[ x <~ y ]] n" := (cas m x y n).
+
+Hint Constructors cas.
+
+Lemma cas_reflexive: forall s x, s [[ x <~ x ]] s.
+Proof.
+  intros s x. induction s.
+  * remember (id_eq_dec i0 x) as Cases. inversion_clear Cases.
+    + subst i0. auto.
+    + auto.
+  * remember (id_eq_dec i0 x) as Cases. inversion_clear Cases.
+    + subst i0. auto.
+    + auto.
+  * auto.
+Qed.
+
+Lemma cas_preserves: forall x y z s s',  z <> x -> z <> y -> s [[x <~ y ]] s' -> fv z s' -> fv z s.
+Proof.
+  intros. induction s0.
+
+Lemma cas_renames_free: forall s s' x y,  x <> y -> s [[ x <~ y ]] s' -> ~fv x s'.
+Proof.
+  induction s0.
+  * intros. remember (id_eq_dec i0 x) as Cases. inversion_clear Cases.
+    + subst i0. intro. inversion H0; subst s'; inversion H1; auto.
+    + inversion H0. intro. inversion H6. auto. intro. inversion H7. auto.
+  * intros. inversion_clear H0.
+    + intro. inversion_clear H0. auto.
+    + intro. inversion_clear H0. apply IHs0 in H3; auto.
+    + remember (id_eq_dec x0 z0) as Cases. inversion_clear Cases.
+      - subst z0. intro. inversion H0. auto.
+      - intro. inversion_clear H4. apply cas_preserves with (x:=y0)(y:=z0)(s:=m') in H5.
+  * intros. inversion_clear H0. intro. inversion_clear H0. inversion_clear H3.
+    + apply IHs0_1 in H1; auto.
+    + apply IHs0_2 in H2; auto.    
+Admitted.
+ *)
+
+Reserved Notation "m [[ x <~ y ]]" (at level 37, left associativity).
+
+Fixpoint rename t x y :=
+  match t with
+  | Var z     => if id_eq_dec z x then v y else t
+  | \ z --> m => if id_eq_dec z x then t else \ z --> m [[x <~ y]]
+  | m @ n     => m [[x <~ y]] @ n [[x <~ y]]
+  end
+where "m [[ x <~ y ]]" := (rename m x y).
+
+(*
+Lemma rename_idempotent: forall s x y, ~fv y s \/ x = y -> rename (rename s x y) y x = s. (* Not true! *)
+Proof. admit. Admitted.
+
+Lemma rename_composition: forall s x y z, ~fv y s -> ~fv z s -> rename (rename s x y) y z = rename s x z. (* Not true! *)
+Proof. admit. Admitted.
+
+Hint Resolve rename_renames_free.
+Hint Resolve rename_idempotent.
+Hint Resolve rename_composition.
+
+Reserved Notation "m ~~> n" (at level 38, no associativity).
+         
+Inductive alpha_convertable : term -> term -> Prop :=
+  ac_Intro : forall x y m n, ~fv y m \/ x = y -> n = rename m x y -> (\ x --> m) ~~> (\ y --> n)
+where "m ~~> n" := (alpha_convertable m n).
+
+Lemma alpha_conversion_reflexive: forall x m, alpha_convertable (\ x --> m) (\x --> m).
+Proof.
+  intros x m. constructor.
+  * right. reflexivity.
+  * induction m.
+    + simpl. destruct (id_eq_dec i0 x); try subst i0; auto. 
+    + simpl. destruct (id_eq_dec i0 x); try rewrite <- IHm; auto.
+    + simpl. rewrite <- IHm1. rewrite <- IHm2. auto.
+Qed.
+
+Lemma alpha_conversion_symmetric: forall m n, alpha_convertable m n -> alpha_convertable n m.
+Proof. admit. Admitted.
+(*
+  intros m n H. inversion_clear H. subst n0. constructor.
+  * inversion_clear H0; [left; auto | right; auto].
+  * symmetry. auto.
+Qed.
+*)
+Lemma alpha_conversion_transitive: forall m n p, alpha_convertable m n -> alpha_convertable n p -> alpha_convertable m p.
+Proof. admit. Admitted.
+(*
+  intros m n p H1 H2. generalize dependent m. generalize dependent n. induction p.
+  * intros. inversion H2.
+  * intros. inversion H2. subst n0. inversion H1. subst m0. constructor.
+    + inversion_clear H8.
+      - left.  subst p. subst m1. auto.
+  * intros. inversion H2.
+Qed.*)
+
+Hint Resolve alpha_conversion_reflexive.
+Hint Resolve alpha_conversion_symmetric.
+Hint Resolve alpha_conversion_transitive.
+
+Reserved Notation "m <~~> n" (at level 38, no associativity).
+
+Inductive alpha_equivalent : term -> term -> Prop :=
+  ae_Base : forall m n      , m ~~> n -> m <~~> n
+| ae_Var  : forall x        , (v x) <~~> (v x)                                    
+| ae_App  : forall m n m' n', m <~~> m' -> n <~~> n' -> (m @ n) <~~> (m' @ n')
+| ae_Lam  : forall x m m'   , m <~~> m' -> \x --> m <~~> \x --> m'
+where "m <~~> n" := (alpha_equivalent m n).
+
+Hint Constructors alpha_equivalent.
+     
+Lemma alpha_equivalence_reflexive: forall m, m <~~> m.
+Proof. intro m. induction m; auto. Qed.
+
+Lemma alpha_equivalence_symmetric: forall m n, m <~~> n -> n <~~> m.
+Proof. intros m n H. induction H; auto. Qed.
+
+Lemma alpha_equivalence_transitive: forall p m n, m <~~> n -> n <~~> p -> m <~~> p.
+Proof.
+  intros p. induction p.
+  * intros. inversion H0.
+    + inversion H1.
+    + subst n0. inversion H0.
+       - inversion H1.
+       - inversion H. inversion H1. auto.
+  * intros. inversion H0.
+    + inversion H1. subst n0. subst m1. inversion H.
+       - apply ae_Base. apply alpha_conversion_transitive with (\ x0 --> m2); auto.
+       - subst x0. subst m0. apply ae_Base. constructor. inversion_clear H7. left. 
+  * intros. inversion H0. inversion H1. subst n0. inversion H. inversion H3.
+    apply ae_App.
+    + apply IHp1 with (m:=m2)(n:=m1); auto.
+    + apply IHp2 with (m:=n0)(n:=n1); auto.
+Admitted.
+ *)
+
+Inductive safe : term -> id -> id -> Prop :=
+  safe_Var   : forall x y z  , x <> z -> safe (Var x) y z
+| safe_App   : forall m n x y, safe m x y -> safe n x y -> safe (m @ n) x y
+| safe_Lam_1 : forall m z y  , safe (\ z --> m) z y
+| safe_Lam_2 : forall m x y z, y <> z -> x <> z -> safe m x y -> safe (\ z --> m) x y
+| safe_Lam_3 : forall m x z  , x <> z -> ~ fv x m -> safe (\ z --> m) x z.
+
+Lemma safe_reverse : forall m x y, safe m x y -> safe (m [[x <~ y]]) y x.
+Proof.
+  intros m x y H. induction m.
+  * simpl. destruct (id_eq_dec i0 x).
+    + subst i0. inversion H. constructor. auto.
+    + inversion H. constructor. auto.
+  * inversion H.
+    + simpl. destruct (id_eq_dec x x). subst x.     
+  * inversion H. simpl. constructor; auto.
+Admitted.
+  
+  * simpl. destruct (id_eq_dec x0 y0).
+    + constructor. subst x0. intro. symmetry in H0. contradiction.
+    + constructor. auto.
+  * simpl. constructor; auto.
+  * 
+   
+  
+
+Hint Resolve safe_reverse.
+
+Lemma rename_reverse : forall m x y, safe m x y -> (m [[x <~ y]]) [[y <~ x]] = m.
+Proof. admit. Admitted.
+
+Hint Resolve rename_reverse.
+
+Reserved Notation "m <~~> n" (at level 38, no associativity).
+
+Inductive alpha_equivalent : term -> term -> Prop :=
+  ae_Var  : forall x, v x <~~> v x
+| ae_App  : forall m n m' n', m <~~> m' -> n <~~> n' -> (m @ n) <~~> (m' @ n')
+| ae_Lam  : forall x m m'   , m <~~> m' -> (\x --> m) <~~> (\x --> m')
+| ae_Conv : forall x y m m' , m <~~> m' -> safe m' x y -> (\x --> m) <~~> (\y --> m' [[x <~ y]])
+where "m <~~> n" := (alpha_equivalent m n).
+
+Hint Constructors alpha_equivalent.
+
+Lemma alpha_reflexive: forall m, m <~~> m.
+Proof. intro m. induction m; auto. Qed.
+
+Hint Resolve alpha_reflexive.
+
+Lemma alpha_transitive: forall m n p,  m <~~> n -> n <~~> p -> m <~~> p.
+Proof. admit. Admitted.
+
+Lemma alpha_symmetric: forall m n, m <~~> n -> n <~~> m.
+Proof.
+  intros m n H. induction H.
+  * auto.
+  * auto.
+  * auto.
+  * assert (M'M0: \ x0 --> m' <~~> \ x0 --> m0). constructor. auto.
+    assert (M0M': \ x0 --> m0 <~~> \ x0 --> m'). constructor. auto.
+    assert (Revr: (m' [[x0 <~ y0]]) [[y0 <~ x0]] = m'). auto.
+    assert (A: \ y0 --> m' [[x0 <~ y0]] <~~> \ x0 --> m'). rewrite <-Revr at 2. constructor; auto.
+    apply alpha_transitive with (\ x0 --> m'); auto. 
+Qed.
