coq/Stmt.v
@@ -60,18 +60,83 @@ Inductive bs_equivalent: stmt -> stmt -> Prop :=
                  (forall (c c' : conf), c == s1 ==> c' <-> c == s2 ==> c') -> s1 ~~~ s2
 where "s1 '~~~' s2" := (bs_equivalent s1 s2).
 
-(* Loops with equivalent bodies are equivalent *)
-Lemma while_eq: forall (e : expr) (s1 s2 : stmt), s1 ~~~ s2 -> WHILE e DO s1 END ~~~ WHILE e DO s2 END.
-Proof.
-  intros. inversion_clear H. constructor. intros. split; (
-    intro; 
-      match goal with 
-        _: _ == WHILE ?e DO ?s END ==> _ |- _ => remember (WHILE e DO s END) as While 
-      end;
-      induction H; try (inversion HeqWhile; subst e0; subst s); [
-        apply bs_While_True with c'; [ assumption | apply H0; assumption | apply IHbs_int2; reflexivity]
-      | apply bs_While_False; assumption]).
-Qed.
+Ltac seq_inversion :=
+  match goal with
+    H: _ == _ ;; _ ==> _ |- _ => inversion_clear H
+  end.
+
+Ltac seq_apply :=
+  match goal with
+  | H: _   == ?s1 ==> ?c' |- _ == (?s1 ;; _) ==> _ => 
+    apply bs_Seq with c'; solve [seq_apply | assumption]
+  | H: ?c' == ?s2 ==>  _  |- _ == (_ ;; ?s2) ==> _ => 
+    apply bs_Seq with c'; solve [seq_apply | assumption]
+  end.
+
+Module SmokeTest.
+
+  (* Associativity of sequential composition *)
+  Lemma seq_assoc : forall (s1 s2 s3 : stmt), 
+                      ((s1 ;; s2) ;; s3) ~~~ (s1 ;; (s2 ;; s3)).
+  Proof.
+    intros s1 s2 s3. constructor. intros c0 c'0. split;
+      intro H; repeat seq_inversion; seq_apply.
+  Qed.
+
+  (* One-step unfolding *)
+  Lemma while_unfolds : forall (e : expr) (s : stmt),
+                          (WHILE e DO s END) ~~~ (COND e THEN s ;; WHILE e DO s END ELSE SKIP END).
+  Proof.
+    intros e s. constructor. intros c0 c'0. split.
+    intro H. inversion_clear H; [ 
+      constructor; [
+        assumption 
+      | apply bs_Seq with (c':=c'); assumption
+      ]
+    | apply bs_If_False; [ assumption | constructor]
+    ].
+    intro H. inversion_clear H; [ 
+      inversion_clear H1; apply bs_While_True with (c':=c'); assumption
+    | destruct c'0; destruct p; inversion H1; apply bs_While_False; subst s0; assumption
+    ].
+  Qed.      
+
+  (* Terminating loop invariant *)
+  Lemma while_false : forall (e : expr) (s : stmt) (st : state Z) (i o : list Z) (c : conf),
+                        c == WHILE e DO s END ==> (st, i, o) -> [| e |] st => Z.zero.
+  Proof.
+    intros. remember (st, i, o). remember (WHILE e DO s END). induction H; solve [
+      inversion Heqs0
+    | inversion Heqs0; subst e0; subst s0; apply IHbs_int2; [assumption | reflexivity]
+    | inversion Heqs0; subst e0; inversion Heqp; subst st0; assumption
+    ].
+  Qed.
+
+  (* Big-step semantics does not distinguish non-termination from stuckness *)
+  Lemma loop_eq_undefined : (WHILE (Nat 1) DO SKIP END) ~~~ (COND (Nat 3) THEN SKIP ELSE SKIP END).
+  Proof.    
+    apply bs_eq_intro. 
+    intros c c'. 
+    split.
+      intro H. destruct c' eqn:C. destruct p eqn:P. 
+        apply (while_false (Nat 1) SKIP s l0 l c) in H. inversion H.
+      intro H. inversion H; inversion H5.
+  Qed.
+
+  (* Loops with equivalent bodies are equivalent *)
+  Lemma while_eq: forall (e : expr) (s1 s2 : stmt), s1 ~~~ s2 -> WHILE e DO s1 END ~~~ WHILE e DO s2 END.
+  Proof.
+    intros. inversion_clear H. constructor. intros. split; (
+      intro; 
+        match goal with 
+          _: _ == WHILE ?e DO ?s END ==> _ |- _ => remember (WHILE e DO s END) as While 
+        end;
+        induction H; try (inversion HeqWhile; subst e0; subst s); [
+          apply bs_While_True with c'; [ assumption | apply H0; assumption | apply IHbs_int2; reflexivity]
+        | apply bs_While_False; assumption]).
+  Qed.
+  
+End SmokeTest.
 
 (* Semantic equivalence is a congruence *)
 Lemma eq_congruence: forall (e : expr) (s s1 s2 : stmt), s1 ~~~ s2 ->
@@ -92,91 +157,30 @@ Proof.
       intro; inversion H; solve [ apply bs_If_True ; solve [assumption | apply H0; assumption]
                                 | apply bs_If_False; solve [assumption | apply H0; assumption]
                                 ]).
-    apply bs_eq_intro in H0. apply while_eq. assumption.      
-Qed.
-
-Ltac seq_inversion :=
-  match goal with
-    H: _ == _ ;; _ ==> _ |- _ => inversion_clear H
-  end.
-
-Ltac seq_apply :=
-  match goal with
-  | H: _   == ?s1 ==> ?c' |- _ == (?s1 ;; _) ==> _ => 
-    apply bs_Seq with c'; solve [seq_apply | assumption]
-  | H: ?c' == ?s2 ==>  _  |- _ == (_ ;; ?s2) ==> _ => 
-    apply bs_Seq with c'; solve [seq_apply | assumption]
-  end.
-
-(* Associativity of sequential composition *)
-Lemma seq_assoc : forall (s1 s2 s3 : stmt), 
-                      ((s1 ;; s2) ;; s3) ~~~ (s1 ;; (s2 ;; s3)).
-Proof.
-  intros s1 s2 s3. constructor. intros c0 c'0. split;
-    intro H; repeat seq_inversion; seq_apply.
-Qed.
-
-(* One-step unfolding *)
-Lemma while_unfolds : forall (e : expr) (s : stmt),
-                        (WHILE e DO s END) ~~~ (COND e THEN s ;; WHILE e DO s END ELSE SKIP END).
-Proof.
-  intros e s. constructor. intros c0 c'0. split.
-    intro H. inversion_clear H; [ 
-      constructor; [
-        assumption 
-      | apply bs_Seq with (c':=c'); assumption
-      ]
-      | apply bs_If_False; [ assumption | constructor]
-    ].
-    intro H. inversion_clear H; [ 
-      inversion_clear H1; apply bs_While_True with (c':=c'); assumption
-    | destruct c'0; destruct p; inversion H1; apply bs_While_False; subst s0; assumption
-    ].
-Qed.      
-
-(* Terminating loop invariant *)
-Lemma while_false : forall (e : expr) (s : stmt) (st : state Z) (i o : list Z) (c : conf),
-                      c == WHILE e DO s END ==> (st, i, o) -> [| e |] st => Z.zero.
-Proof.
-  intros. remember (st, i, o). remember (WHILE e DO s END). induction H; solve [
-    inversion Heqs0
-  | inversion Heqs0; subst e0; subst s0; apply IHbs_int2; [assumption | reflexivity]
-  | inversion Heqs0; subst e0; inversion Heqp; subst st0; assumption
-  ].
-Qed.
-
-(* Big-step semantics does not distinguish non-termination from stuckness *)
-Lemma loop_eq_undefined : (WHILE (Nat 1) DO SKIP END) ~~~ (COND (Nat 3) THEN SKIP ELSE SKIP END).
-Proof.    
-  apply bs_eq_intro. 
-  intros c c'. 
-  split.
-    intro H. destruct c' eqn:C. destruct p eqn:P. 
-      apply (while_false (Nat 1) SKIP s l0 l c) in H. inversion H.
-    intro H. inversion H; inversion H5.
+    apply bs_eq_intro in H0. apply SmokeTest.while_eq. assumption.      
 Qed.
 
 (* Big-step semantics is deterministic *)
-Ltac by_bs_eval_deterministic :=
+Ltac by_eval_deterministic :=
   match goal with
     H1: [|?e|]?s => ?z1, H2: [|?e|]?s => ?z2 |- _ => 
-     apply (bs_eval_deterministic e s z1 z2) in H1; [subst z2; reflexivity | assumption]
+     apply (eval_deterministic e s z1 z2) in H1; [subst z2; reflexivity | assumption]
   end.
 
 Lemma bs_int_deterministic : forall (c c1 c2 : conf) (s : stmt), c == s ==> c1 -> c == s ==> c2 -> c1 = c2.
 Proof. 
   intros c c1 c2 s H. revert c2. induction H.
     intros c2 H1. inversion H1. reflexivity.
-    intros c2 H1. inversion H1. by_bs_eval_deterministic.
+    intros c2 H1. inversion H1. by_eval_deterministic.
     intros c2 H1. inversion H1. reflexivity.
-    intros c2 H1. inversion H1. by_bs_eval_deterministic.
+    intros c2 H1. inversion H1. by_eval_deterministic.
     intros c2 H1. inversion H1. apply IHbs_int1 in H4. subst c'0. apply IHbs_int2 in H7. assumption.
-    intros c2 H1. inversion H1. apply IHbs_int in H10. assumption. apply bs_eval_deterministic with (z1 := Z.zero) in H. inversion H. assumption.
-    intros c2 H1. inversion H1. apply bs_eval_deterministic with (z1 := Z.one) in H. inversion H. assumption.
+    intros c2 H1. inversion H1. apply IHbs_int in H10. assumption. apply eval_deterministic with (z1 := Z.zero) in H. inversion H. assumption.
+    intros c2 H1. inversion H1. apply eval_deterministic with (z1 := Z.one) in H. inversion H. assumption.
       apply IHbs_int in H10. assumption.
     intros c2 H2. inversion H2. apply IHbs_int1 in H10. subst c'0. apply IHbs_int2 in H11. assumption.
-      apply bs_eval_deterministic with (z2 := Z.one) in H9. inversion H9. assumption.
-    intros c2 H1. inversion H1. apply bs_eval_deterministic with (z1 := Z.one) in H. inversion H. assumption.
+      apply eval_deterministic with (z2 := Z.one) in H9. inversion H9. assumption.
+    intros c2 H1. inversion H1. apply eval_deterministic with (z1 := Z.one) in H. inversion H. assumption.
       reflexivity.
 Qed.
 
@@ -223,10 +227,139 @@ Proof.
       unfold plug; assumption
     | simpl; by_eq_congruence (Nat 0) s (C <~ s1) (C <~ s2) IHC
     | simpl; by_eq_congruence e s (C <~ s1) (C <~ s2) IHC
-    | simpl; apply while_eq; assumption
+    | simpl; apply SmokeTest.while_eq; assumption
     ].
     intro H. inversion H. remember (H0 Hole) as C. unfold plug in C. assumption.
 Qed.
+
+(* Small-step semantics *)
+Module SmallStep.
+  
+  Reserved Notation "c1 '--' s '-->' c2" (at level 0).
+
+  Inductive ss_int_step : stmt -> conf -> option stmt * conf -> Prop :=
+  | ss_Skip        : forall (c : conf), c -- SKIP --> (None, c) 
+  | ss_Assign      : forall (s : state Z) (i o : list Z) (x : id) (e : expr) (z : Z), 
+                       [| e |] s => z -> (s, i, o) -- x ::= e --> (None, (s [x <- z], i, o))
+  | ss_Read        : forall (s : state Z) (i o : list Z) (x : id) (z : Z),
+                       (s, z::i, o) -- READ x --> (None, (s [x <- z], i, o))
+  | ss_Write       : forall (s : state Z) (i o : list Z) (e : expr) (z : Z), 
+                       [| e |] s => z -> (s, i, o) -- WRITE e --> (None, (s, i, z::o))
+  | ss_Seq_Compl   : forall (c c' : conf) (s1 s2 : stmt),
+                       c -- s1 --> (None, c') -> c -- s1 ;; s2 --> (Some s2, c')
+  | ss_Seq_InCompl : forall (c c' : conf) (s1 s2 s1' : stmt),
+                       c -- s1 --> (Some s1', c') -> c -- s1 ;; s2 --> (Some (s1' ;; s2), c')
+  | ss_If_True     : forall (s : state Z) (i o : list Z) (s1 s2 : stmt) (e : expr),
+                       [| e |] s => Z.one -> (s, i, o) -- COND e THEN s1 ELSE s2 END --> (Some s1, (s, i, o))
+  | ss_If_False    : forall (s : state Z) (i o : list Z) (s1 s2 : stmt) (e : expr),
+                       [| e |] s => Z.zero -> (s, i, o) -- COND e THEN s1 ELSE s2 END --> (Some s2, (s, i, o))
+  | ss_While       : forall (c : conf) (s : stmt) (e : expr),
+                       c -- WHILE e DO s END --> (Some (COND e THEN s ;; WHILE e DO s END ELSE SKIP END), c)
+  where "c1 -- s --> c2" := (ss_int_step s c1 c2).
+
+  Reserved Notation "c1 '--' s '-->>' c2" (at level 0).
+
+  Inductive ss_int : stmt -> conf -> conf -> Prop :=
+    ss_int_Base : forall (s : stmt) (c c' : conf),
+                    c -- s --> (None, c') -> c -- s -->> c'
+  | ss_int_Step : forall (s s' : stmt) (c c' c'' : conf),
+                    c -- s --> (Some s', c') -> c' -- s' -->> c'' -> c -- s -->> c'' 
+  where "c1 -- s -->> c2" := (ss_int s c1 c2).
+
+  Lemma ss_int_step_deterministic :
+    forall (c : conf) (c' c'' : option stmt * conf) (s : stmt),
+      c -- s --> c' -> c -- s --> c'' -> c' = c''.
+  Proof.
+    intros. generalize dependent c'. generalize dependent c''. generalize dependent c. induction s.
+    * intros. inversion H. inversion H0. auto.
+    * intros. inversion H. inversion H0.
+      rewrite <-H2 in H7. inversion H7. subst.
+      apply eval_deterministic with (z1:=z0) in H5; try auto; subst; auto.
+    * intros. inversion H. inversion H0. rewrite <-H1 in H4. inversion H4. auto.
+    * intros. inversion H. inversion H0. subst c. inversion H7. subst s0. apply eval_deterministic with (z1:=z) in H6. subst z0. reflexivity. auto.
+    * intros. inversion H0.
+        inversion H.
+          apply (IHs1 c (None, c'0)) in H10. inversion H10; auto. auto.
+          apply (IHs1 c (None, c'0)) in H10. inversion H10. auto.
+        inversion H.
+          apply (IHs1 c (Some s1', c'0)) in H10. inversion H10. auto.
+          apply (IHs1 c (Some s1', c'0)) in H10. inversion H10. auto. auto.
+    * intros. inversion H0.
+      + inversion H.
+         - subst c. inversion H8. auto.
+         - subst c. inversion H8. subst s4. apply eval_deterministic with (z1:=Z.one) in H12. inversion H12. assumption.
+      + inversion H.
+         - subst c. inversion H8. subst s4. apply eval_deterministic with (z1:=Z.one) in H6. inversion H6. assumption.
+         - subst c. inversion H8. auto.
+    * intros. inversion H0. inversion H. auto.
+  Qed.
+
+  Lemma ss_int_deterministic : forall (c c' c'' : conf) (s : stmt),  c -- s -->> c' -> c -- s -->> c'' -> c' = c''.
+  Proof.
+    intros. generalize dependent c'. induction H0.
+    * intros. inversion H0.
+        apply ss_int_step_deterministic with (c':=(None, c')) in H1. inversion H1; auto. auto.
+        apply ss_int_step_deterministic with (c':=(None, c')) in H1. inversion H1; auto. auto.
+    * intros. inversion_clear H1.
+        apply ss_int_step_deterministic with (c':=(Some s', c')) in H2. inversion H2; auto. auto.
+        apply ss_int_step_deterministic with (c':=(Some s'0, c'1)) in H. inversion H. subst; auto. auto.
+  Qed.
+  
+  Lemma ss_bs_base : forall (s : stmt) (c c' : conf),  c -- s --> (None, c') -> c == s ==> c'.
+  Proof.
+    intros. inversion H; constructor; auto.
+  Qed.
+
+  Lemma ss_ss_composition :
+    forall (c c' c'' : conf) (s1 s2 : stmt), c -- s1 -->> c'' -> c'' -- s2 -->> c' -> c -- s1 ;; s2 -->> c'. 
+  Proof.
+    intros. induction H.
+    * inversion H.
+      + apply ss_int_Step with (s':=s2)(c':=c'0). constructor. subst c'0. subst s. subst c. assumption. assumption.
+      + apply ss_int_Step with (s':=s2)(c':=c'0). constructor. subst c'0. subst s. subst c. assumption. assumption.
+      + apply ss_int_Step with (s':=s2)(c':=c'0). constructor. subst c'0. subst s. subst c. assumption. assumption.
+      + apply ss_int_Step with (s':=s2)(c':=c'0). constructor. subst c'0. subst s. subst c. assumption. assumption.
+        * assert (A: c -- s;; s2 --> (Some (s';;s2), c'0)).
+           constructor. assumption.            
+      apply ss_int_Step with (s':=s';;s2)(c':=c'0). assumption. apply IHss_int in H0. assumption.
+  Qed.
+  
+  Lemma ss_bs_step :
+    forall (c c' c'' : conf) (s s' : stmt), c -- s --> (Some s', c') -> c' == s' ==> c'' -> c == s ==> c''.
+  Proof.
+    intros.
+      generalize dependent c.
+      generalize dependent c'.
+      generalize dependent c''.
+      generalize dependent s'.
+      induction s; intros; inversion H.
+      * apply ss_bs_base in H4. apply bs_Seq with (c':=c'); auto.
+      * subst s'. inversion H0. specialize (IHs1 s1' c'1 c' H8 c H4). apply bs_Seq with (c':=c'1); auto.
+      * apply bs_If_True; auto. subst c'. auto.
+      * apply bs_If_False; auto. subst c'. auto.
+      * remember (SmokeTest.while_unfolds e s). inversion_clear b. apply H4. subst. auto.
+  Qed.  
+
+  Theorem bs_ss_eq : forall (s : stmt) (c c' : conf),  c == s ==> c' <-> c -- s -->> c'.
+  Proof.
+    intros. split.
+    * intro. induction H.
+      + repeat constructor.
+      + repeat constructor. auto.
+      + repeat constructor.
+      + repeat constructor. auto.
+      + eapply ss_ss_composition; eauto.
+      + eapply ss_int_Step. apply ss_If_True; auto. auto.
+      + eapply ss_int_Step. apply ss_If_False; auto. auto.
+      + eapply ss_int_Step. apply ss_While. eapply ss_int_Step. apply ss_If_True; auto. eapply ss_ss_composition; eauto.
+      + eapply ss_int_Step. apply ss_While. apply ss_int_Step with (s':=SKIP)(c':=(st, i, o)). apply ss_If_False. auto.
+        apply ss_int_Base. apply ss_Skip.
+    * intro. induction H.
+      + inversion_clear H; constructor; auto.
+      + apply ss_bs_step with (c':=c')(s':=s'); auto.
+  Qed.
+  
+End SmallStep.
 
 (* CPS semantics *)
 Inductive cont : Type := 
@@ -281,7 +414,6 @@ Inductive cps_int : cont -> cont -> conf -> conf -> Prop :=
                       KEmpty |- (st, i, o) -- k --> c' ->
                       k |- (st, i, o) -- !(WHILE e DO s END) --> c'
 where "k |- c1 -- s --> c2" := (cps_int k s c1 c2).
-
     
 Lemma cps_bs_gen: forall (S : stmt) (c c' : conf) (S1 k : cont),
                 k |- c -- S1 --> c' -> !S = S1 @ k -> c == S ==> c'.
@@ -311,7 +443,7 @@ Proof.
     intros. 
       destruct k eqn:K. 
         unfold Kapp in *. inversion H0. apply IHcps_int. reflexivity. 
-        unfold Kapp in *. inversion H0. remember (seq_assoc s1 s2 s) as Hassoc.
+        unfold Kapp in *. inversion H0. remember (SmokeTest.seq_assoc s1 s2 s) as Hassoc.
           inversion Hassoc. apply H1. apply IHcps_int. reflexivity.
     intros. 
       destruct k eqn:K. 
@@ -332,7 +464,7 @@ Proof.
           apply A. assumption. apply IHcps_int. reflexivity.
     intros. 
       destruct k eqn:K. 
-        unfold Kapp in *. inversion H1. remember (while_unfolds e s) as Hunfold.
+        unfold Kapp in *. inversion H1. remember (SmokeTest.while_unfolds e s) as Hunfold.
           inversion Hunfold. apply H2. apply bs_If_True. assumption. apply IHcps_int. reflexivity.
         unfold Kapp in *. inversion H1. 
           assert (A: forall (e : expr) (s s0 : stmt) (st : state Z) (i o : list Z) (c' : conf),
@@ -387,7 +519,7 @@ Qed.
 Lemma cps_seq_gen: forall (E k S1 : cont) (s1 s2 : stmt) (c c' c'' : conf),
                  k |- c -- S1 --> c' -> S1 = !s1 -> KEmpty |- c' -- !s2 --> c'' -> k @ !s2 |- c -- S1 --> c''.
 Proof. admit.
-Qed.
+Admitted.
 
 Lemma cps_seq: forall (k : cont) (s1 s2 : stmt) (c c' c'' : conf),
                  k |- c -- !s1 --> c' -> KEmpty |- c' -- !s2 --> c'' -> k @ !s2 |- c -- !s1 --> c''.
@@ -412,7 +544,7 @@ Proof.
     apply cps_While_True. assumption. unfold Kapp.
       rewrite (A (WHILE e DO s END)). apply cps_seq with c'; assumption.
     apply cps_While_False. assumption. constructor.
-Qed.
+Admitted.
 
     
 
